Update specs to use new lib

specs/Spec.Ed25519.fst
@@ -10,7 +10,6 @@ open Spec.Curve25519
 
 module BF = Vale.Arch.BufferFriend
 
-
 #reset-options "--max_fuel 0 --z3rlimit 100"
 
 ///
@@ -49,8 +48,9 @@ let g: ext_point = (g_x, g_y, 1, g_x *% g_y)
 let modp_inv (x:elem) : Tot elem =
   x **% (prime - 2)
 
-let sha512_modq (len:size_nat) (s:lbytes len) : (n:nat{n < pow2 256}) =
+let sha512_modq (len:size_nat) (s:lbytes len) : n:nat{n < pow2 256} =
   nat_from_bytes_le (BF.to_bytes (Spec.Hash.hash Spec.Hash.Definitions.SHA2_512 (BF.of_bytes s))) % q
+
 
 let point_add (p:ext_point) (q:ext_point) : Tot ext_point =
   let x1, y1, z1, t1 = p in
@@ -161,23 +161,36 @@ let point_equal (p:ext_point) (q:ext_point) =
 /// Ed25519 API
 ///
 
+let expand_keys (secret: lbytes 32) : (lbytes 32 & lbytes 32 & lbytes 32) =
+  let s, prefix = secret_expand secret in
+  let pub = secret_to_public secret in
+  pub, s, prefix
+
+val sign_expanded:
+  pub:lbytes 32 ->
+  s:lbytes 32 ->
+  prefix:lbytes 32 ->
+  msg: bytes{64 + length msg <= max_size_t} ->
+  Tot (lbytes 64)
+let sign_expanded pub s prefix msg =
+  let len = length msg in
+  let r = sha512_modq (32 + len) (concat #uint8 #32 #(length msg) prefix msg) in
+  let r' = point_mul (nat_to_bytes_le 32 r) g in
+  let rs = point_compress r' in
+  let h = sha512_modq (64 + len)
+    (concat #uint8 #64 #(length msg) (concat #uint8 #32 #32 rs pub) msg)
+  in
+  let s = (r + (h * nat_from_bytes_le s) % q) % q in
+  concat #uint8 #32 #32 rs (nat_to_bytes_le 32 s)
+
 val sign:
     secret: lbytes 32
   -> msg: bytes{64 + length msg <= max_size_t} ->
   Tot (lbytes 64)
 
 let sign secret msg =
-  let len = length msg in
-  let a, prefix = secret_expand secret in
-  let a' = point_compress (point_mul a g) in
-  let r = sha512_modq (32 + len) (concat #uint8 #32 #(length msg) prefix msg) in
-  let r' = point_mul (nat_to_bytes_le 32 r) g in
-  let rs = point_compress r' in
-  let h = sha512_modq (64 + len)
-    (concat #uint8 #64 #(length msg) (concat #uint8 #32 #32 rs a') msg)
-  in
-  let s = (r + (h * nat_from_bytes_le a) % q) % q in
-  concat #uint8 #32 #32 rs (nat_to_bytes_le 32 s)
+  let pub, s, prefix = expand_keys secret in
+  sign_expanded pub s prefix msg
 
 val verify:
     public: lbytes 32
